LeanProjeto2/ShoenfieldsFunctInterp.lean
@@ -10,143 +10,388 @@ open LFormula
 open StarLang
 --open FType
 
+/- EXEMPLO BASE (a tirar depois)
+--import LeanProjeto2.FOL
+--open FOL
+--open LFormula
+example
+  (hA1 : SH_int A AuSH) (hA2 : AuSH.components = (a,b,A_SH)) (hA3 : StarLang.isBase A_SH)
+  (hB1 : SH_int B BuSH) (hB2 : BuSH.components = (c,d,B_SH)) (hB3 : StarLang.isBase B_SH) :
+  (SH_int (  ) (Recreate ( , , ))) := by sorry
+-/
+
+
 -- SHOENFIELD'S FUNCTIONAL INTERPREATION
 
 -- ---------------------------------------------------------------------------------------------------------------
 --             SECTION 2.2: Shoenfield's functional interpretation
 -- ---------------------------------------------------------------------------------------------------------------
 
-
 -- -------------------------------------------------------------
--- DEFINITION 2.1 (p.40): Shoenfield's functional interpretation
+-- DEFINITION 2.1 (p.38): Shoenfield's functional interpretation
 -- -------------------------------------------------------------
 
 /-
-A^SH = ∀a ∃b A_SH (a,b) : Formula    ->    (A^ -> V a E b A_)
-B^SH = ∀c ∃d B_SH (c,d) : Formula    ->    (B^ -> V c E d B_)
+To define Shoenfield's functional interpretation we need some auxiliary functions to deal with the
+different components of the interpretation of a formula. Every interpretation has a list of universal
+variables, a list of existential variables and the matrix, i.e. the lower SH-formula (a base formula).
+These three components will be represented by a tuple.
 
-def SH_int : Formula → Formula
-| SH_base
-| SH_or
-| SH_not
-| SH_unb_forall
-| SH_b_forall
+For example, if a formula A has the interpretation A^SH given by
+                        ∀a ∃b A_SH(a,b)
+then we would represent this as (a,b,A_SH).
 
-def SH_int : Finset Term.var → Finset Term.var → Formula → Formula            -- TO DO: Precisamos do ∀₁ para tuples of variables
-| SH_base
-| SH_or
-| SH_not
-| SH_unb_forall
-| SH_b_forall
+The function 'components' transforms a formula such as ∀a ∃b A_SH(a,b) into the tupe (a,b,A_SH).
+The function 'Recreate' transforms a tuple such as (a,b,A_SH) into the formula ∀a ∃b A_SH(a,b).
 
-def SH_int : Formula → Formula                              LISTAS DE VAR UNIV E VAR EXIST? List Term → List Term → Formula → Formula
-| SH_base
-    | (isBase A) => A
-| V a E b A_ , V c E d B_ => V a V c E b E d (A_ ∨₁ B_)
-    | {a} {b} A_ , c d B_ => {a c} {b d} (A_ ∨₁ B_)         USAR APPEND DAS LISTAS?
-| SH_not
-    | {a} {b} A_ =>                                         COMO CRIAR f a partir de b e a' a partir de a???
-                                                            acho que precisamos de usar substitution
-| SH_unb_forall
-| SH_b_forall
-
-def interp : Formula → Formula
-| SH_base: (isBase A) => A
-
-
-
-
-def SH_int : Formula → Formula
-| Formula.lcons p ts => Formula.lcons p ts
-| Formula.not A =>
-  Formula.forall_L "f" (Formula.exists_L "a'" (Formula.not_L (subst_formula "a" (LTerm.Lfunc "f" [LTerm.Lvar "a"]) (SH_int A))))
-| Formula.or A B =>
-  let A_SH := SH_int A in
-  let B_SH := SH_int B in
-  Formula.forall_L "a" (Formula.exists_L "b" (subst_formula "a" (LTerm.Lvar "b") A_SH)) ∧
-  Formula.forall_L "c" (Formula.exists_L "d" (subst_formula "c" (LTerm.Lvar "d") B_SH)) →
-  Formula.forall_L "a" (Formula.forall_L "c" (Formula.exists_L "b" (Formula.exists_L "d" (Formula.or_L (subst_formula "a" (LTerm.Lvar "b") A_SH) (subst_formula "c" (LTerm.Lvar "d") B_SH)))))
-| Formula.bForall x A =>
-  let A_SH := SH_int A in
-  Formula.forall_L x (Formula.forall_L "a" (Formula.exists_L "b" (subst_formula x (LTerm.Lvar "a") A_SH)))
-| Formula.exists_L x A =>
-  let A_SH := SH_int A in
-  Formula.forall_L "a" (Formula.exists_L "b" (Formula.exists_L x (subst_formula x (LTerm.Lvar "a") A_SH)))
-| Formula.bounded_forall_L x t A =>
-  let A_SH := SH_int A in
-  Formula.forall_L "a" (Formula.exists_L "b" (Formula.forall_L x (Formula.and_L (Formula.atomic_L "in" [LTerm.Lvar x, t]) (subst_formula x (LTerm.Lvar "a") A_SH))))
-
---inductive SHint : Finset String → Finset String → Formula → Formula
---| sorry
-
-def SH_int2 : Formula → Formula
-| Formula.or A B =>
-  V₁ "a" (E₁ "b" (substitution_formula "a" (Term.var "b") A_SH)) →
-  V₁ "c" (E₁ "d" (substitution_formula "c" (Term.var "d") B_SH)) →
-  V₁ "a" (V₁ "c" (E₁ "b" (E₁ "d" ((substitution_formula "a" (Term.var "b") A_SH) ∨₁ (substitution_formula "c" (Term.var "d") B_SH)))))
-
+The function 'components_neg' is to deal with the negation.
 -/
-
-
---inductive SH_int : Formula → Formula
---| SH_base (h: isBase A) A : SH_int
-
---def SH_int (α β : Finset String) (A : Formula) : Formula := ∀ α, ∃ β
-
--- TO DO: como falar das lower SH-formulas?
 
 namespace StarLang.Formula
 
+-- AUXILIARY FUNCTIONS:
+-- TO DO / Problema : components não pode ser feito usando ∃ diretamente? Não, é o pattermatching
+
+/-
 def components_neg : Formula → (Finset String × Finset String × Formula)
 | .unbForall x F => let (a,b,rest) := components_neg F;
                     (a,{x} ∪ b,rest)
 | F => ({},{},F)
+-/
 
 def components : Formula → (Finset String × Finset String × Formula)
+-- Reunião: daria se calhar para pôr aqui um not e forall
 | .unbForall x F => let (a,b,rest) := components F;
                     ({x} ∪ a,b,rest)
-| .not F => components_neg F
+| .not (.unbForall x F) => let (a,b,rest) := components F;
+                           (a,{x} ∪ b,rest)
+| .not F => components F
 | F => ({},{},F)
+-- Só se pode usar quando ja estiver com ∀a ∃b
+
+-- Example to use components
+def A_teste : Formula := Formula.rel "R" []
+def exampleFormula : Formula :=
+  bV₁ "x" (Term.var "t") (¬₁ (V₁ "y" A_teste))
+#eval exampleFormula.components  -- Devia dar ({x}, {y}, A_teste), mas falta Repr -- TO DO / Problema
+
+def formula_teste (A:Formula) : Formula := (V₁ "x" (E₁ "y" (E₁ "z" (¬₁A))))
+#eval (formula_teste A_teste).components -- Devia dar ({x}, {y, z}, ¬₁A), mas falta Repr -- TO DO / Problema
+
+-- ∀ a ∃ b [¬ (b∀)]
+
+-- ∀ a ∃ b -> (a,b,...) --> b∀₁ a
+
 
 end StarLang.Formula
 
 noncomputable def recreate : (Finset String × Finset String × Formula) → Formula
-| (a,b,rest) => let ex := List.foldl (fun f x => .not (.unbForall x f)) rest (b.val.toList : List String)
+| (a,b,rest) => -- Problema: Assim ficamos com (x,y,¬F) em vez de (x,y,F)
+                let ex := List.foldl (fun f x => .not (.unbForall x f)) rest (b.val.toList : List String)
                 List.foldl (fun f x => .unbForall x f) ex (a.val.toList : List String)
 
-inductive SH_int : Formula → Formula → Prop                 -- TO DO: ok but how can I make computations?
-| base : (h : StarLang.isBase A) → SH_int A A               -- TO DO: Doesn't capture the essence...
-| disj : SH_int A AuSH →
+noncomputable def Recreate : (Finset String × Finset String × Formula) → Formula
+| (a, b, rest) => -- Assim já ficamos com (x,y,F)
+  -- Negações dentro do b
+                let neg := List.foldl (fun f x => .unbForall x (.not f)) rest (b.val.toList : List String)
+  -- unbForall dentro do a
+                List.foldl (fun f x => .unbForall x f) neg (a.val.toList : List String)
+-- TO DO / Problema: dá para acrescentar aqui que rest is always base? Fazer lema (Reunião)
+
+-- --------------------------------------
+-- DEFINITION 2.1 (p.38):
+-- Shoenfield's functional interpretation
+-- --------------------------------------
+
+/-
+Here we will represent an interpretation A^SH such as ∀a∃b A_SH(a,b) as
+                  ( SH_int A^SH ( Recreate (a,b,A_SH) ) )
+              ( SH_int upperSH ( Recreate (univ_var,exist_var,lowerSH) ) )
+-/
+
+-- TODO / Problema: variaveis disjuntas -> Reunião: na documentação ver se Finset já tem disjunto
+-- a∪b∪c∪d : Finset     -> ver Disjoint a b c d
+inductive SH_int : Formula → Formula → Prop
+| base : (h : StarLang.isBase A) → (SH_int A (Recreate ({},{},A)))
+| disj : SH_int A AuSH →          -- TODO: isto é preciso?
          SH_int B BuSH →
-         AuSH.components = (a,b,A_SH) →
-         BuSH.components = (c,d,B_SH) →
-         --({a,b} ⊆ A.allvars) →
-         -- TODO: dizer lista não tem conjuntos repetidos
-         --({c,d} ⊆ B.allvars) →
-         --(SH_int A (V₁ a (E₁ b A_SH))) →
-         --(SH_int B (V₁ c (E₁ d B_SH))) →
-         (hA : StarLang.isBase A_SH) →                                      -- A^SH = ∀a ∃b A_SH(a,b)
-         (hB : StarLang.isBase B_SH) →                                      -- B^SH = ∀c ∃d B_SH(c,d)
-         (SH_int (A∨₁B) (recreate (a∪c,b∪d,(A_SH ∨₁ B_SH))))
-         --(SH_int (A∨₁B) (V₁ a (V₁ c (E₁ b (E₁ d (A_SH ∨₁ B_SH))))))         -- (A∨B)^SH = ∀a,c ∃b,d [ A_SH(a,b) ∨ B_SH(c,d) ]
-| neg {f:String}: ({a,b} ⊆ A.allvars) →
-        (SH_int A (V₁ a (E₁ b A_SH))) →                                     -- A^SH = ∀a ∃b A_SH(a,b)
+         AuSH.components = (a,b,A_SH) →                                     -- A^SH = ∀a ∃b A_SH(a,b)
+         BuSH.components = (c,d,B_SH) →                                     -- B^SH = ∀c ∃d B_SH(c,d)
+         --({a,b} ⊆ A.allvars) →                                            -- TO DO: precisamos?
+         --({c,d} ⊆ B.allvars) →                                            -- TO DO: dizer lista não tem conjuntos repetidos
+         (hA : StarLang.isBase A_SH) →
+         (hB : StarLang.isBase B_SH) →
+         (SH_int (A∨₁B) (Recreate (a∪c,b∪d,(A_SH ∨₁ B_SH))))                -- (A∨B)^SH = ∀a,c ∃b,d [ A_SH(a,b) ∨ B_SH(c,d) ]
+| neg {f a':String}:
+        -- ({a,b} ⊆ A.allvars) →
+        SH_int A AuSH →
+        AuSH.components = (a,b,A_SH) →                                     -- A^SH = ∀a ∃b A_SH(a,b)
         (hA : StarLang.isBase A_SH) →
-        ((SH_int (¬₁A) (V₁ f (E₁ a' (bE₁ a (Term.var (a')) (¬₁(substitution_formula b ((Term.var f)·(Term.var a)) A_SH)))))))   -- (¬A)^SH = ∀f ∃a' [ ∃a∈a' ¬A_SH(a,fa) ]
-| unbForall : ({x,a,b} ⊆ A.allvars) →
-              (SH_int A (V₁ a (E₁ b A_SH))) →                               -- A^SH = ∀a ∃b A_SH(a,b)
+        (SH_int (¬₁A) (Recreate (b,b,A_SH)))  -- TODO: apagar porque foi batota
+        --(SH_int (¬₁A) (Recreate ({f},{a'},(bE₁ a (Term.var a') (¬₁(substitution_formula b ((Term.var f)·(Term.var a)) A_SH))))))      -- TO DO / Problema: problema: o bE₁ devia então aceitar Finset String :'(
+        --((SH_int (¬₁A) (V₁ f (E₁ a' (bE₁ a (Term.var (a')) (¬₁(substitution_formula b ((Term.var f)·(Term.var a)) A_SH)))))))         -- (¬A)^SH = ∀f ∃a' [ ∃a∈a' ¬A_SH(a,fa) ]
+| unbForall : SH_int A AuSH →
+              AuSH.components = (a,b,A_SH) →                                -- A^SH = ∀a ∃b A_SH(a,b)
+              --({x,a,b} ⊆ A.allvars) →
+              --(SH_int A (V₁ a (E₁ b A_SH))) →                             -- A^SH = ∀a ∃b A_SH(a,b)
               (hA : StarLang.isBase A_SH) →
-              (SH_int (V₁ x A) (V₁ x (V₁ a (E₁ b A_SH))))                   -- (∀x A)^SH = ∀x,a ∃b [ A_SH(x,a,b) ]
-| bForall : ({x,a,b} ⊆ A.allvars) →
-            -- (h : x ∉ t.freevars)
-            (SH_int A (V₁ a (E₁ b A_SH))) →                                 -- A^SH = ∀a ∃b A_SH(a,b)
+              (SH_int (V₁ x A) (Recreate (a∪{x},b,A_SH)))                   -- (∀x A)^SH = ∀x,a ∃b [ A_SH(x,a,b) ]
+| bForall : SH_int A AuSH →
+            AuSH.components = (a,b,A_SH) →                                -- A^SH = ∀a ∃b A_SH(a,b)
             (hA : StarLang.isBase A_SH) →
-            (SH_int (bV₁ x t A) (V₁ a (E₁ b (bV₁ x t A_SH))))               -- (∀x∈t A(x))^SH = ∀a ∃b [ ∀x∈t A_SH(x,a,b) ]
+            (SH_int (bV₁ x t A) (Recreate (a,b,(bV₁ x t A_SH))))
+            --({x,a,b} ⊆ A.allvars) →
+            --(h : x ∉ t.freevars)
+            --(SH_int A (V₁ a (E₁ b A_SH))) →                                 -- A^SH = ∀a ∃b A_SH(a,b)
+            --(SH_int (bV₁ x t A) (V₁ a (E₁ b (bV₁ x t A_SH))))               -- (∀x∈t A(x))^SH = ∀a ∃b [ ∀x∈t A_SH(x,a,b) ]
 
--- função com
-
+-- TO DO (eu): a tirar este Teste e fazer um melhor
 def Teste (a b : String) (f : Term) (A_SH : Formula): Formula := substitution_formula b (f·(Term.var a)) A_SH
--- TO DO no: mudar def de substitution para que sejam Term.var em vez de String
--- TODO: variaveis disjuntas
 
--- TO DO yes: falta substituição + Why V₁ f not working and diz que é term?
+-- --------------------------------------------------------------
+-- EXAMPLE 2.1 (p.38)
+-- Interpretation of (A ∨ (∀x∈t B(x))), with B(x) a base formula.
+-- --------------------------------------------------------------
+
+/-
+SH_int A AuSH
+AuSH.components = (a,b,A_SH)
+(hA : StarLang.isBase A_SH)
+
+SH_int B BuSH
+BuSH.components = ({},{},B_SH)
+(hB : StarLang.isBase B)        -- usar aqui SH_int.base para obter: SH_int B (Recreate ({},{},B))
+
+TO SHOW:
+(SH_int ( A ∨₁ (bV₁ x t B) ) (Recreate (a,b,( A_SH ∨₁ (bV₁ x t B_SH) ))))
+
+-/
+
+example
+  (hA1 : SH_int A AuSH) (hA2 : AuSH.components = (a,b,A_SH)) (hA3 : StarLang.isBase A_SH)
+  (hB1 : SH_int B BuSH) (hB2 : BuSH.components = ({},{},B_SH)) (hB3 : StarLang.isBase B_SH) :
+  (SH_int ( A ∨₁ (bV₁ x t B) ) (Recreate (a,b,( A_SH ∨₁ (bV₁ x t B_SH) )))) :=
+  by
+    have H := SH_int.base hB3   -- Recreate dá: SH_int B_SH (Recreate (∅, ∅, B_SH))
+    -- Mostrar que (bV₁ x t B_SH) isBase
+    -- | b_bForall (x : String) (t : Term) (h : isBase A) : isBase (bForall x t A)
+    have H2 := StarLang.isBase.b_bForall x t hB3        -- H2 : isBase (bV₁ x t B_SH)
+    -- Agora queremos a interpretação do ∨ para termos a interpretação de (A ∨ (∀x∈t B(x)))
+    -- Definir a fórmula:
+    let F := Formula.bForall x t B_SH
+    sorry
+    /-
+    have H1 : {x} = F.components.1 :=
+      by unfold Formula.components
+         simp
+    have H : (x', t', B_SH') = F.components := by sorry       -- Problema: como garantir que F.components spits the right tuple?
+    sorry
+    --let cF : Finset String × Finset String × Formula := F.components
+    -/
+
+-- ---------------------------------------------------------------------
+-- EXAMPLE 2.2 (p.38)                           -- TO DO: depois de termos resolvido a negação do SH_int
+-- Interpretation of ∀y∈t ¬(∃x ¬A(x) ∧ B(y)).
+-- ---------------------------------------------------------------------
+
+/-
+SH_int A AuSH
+AuSH.components = (a,b,A_SH)
+(hA : StarLang.isBase A_SH)
+
+SH_int B BuSH
+BuSH.components = (c,d,B_SH)
+(hB : StarLang.isBase B_SH)
+
+TO SHOW:
+(SH_int ( bV₁ y t ( ¬₁((E₁ x A)∧₁B) ) ) (Recreate ({x}∪a∪g,b∪(c'),( bV₁ y t (A_SH ∨₁ (bE₁ c c' (substitution_formula d ((Term.var g)·(Term.var c)) B_SH)   )) ))))
+
+example
+  (hA1 : SH_int A AuSH) (hA2 : AuSH.components = (a,b,A_SH)) (hA3 : StarLang.isBase A_SH)
+  (hB1 : SH_int B BuSH) (hB2 : BuSH.components = (c,d,B_SH)) (hB3 : StarLang.isBase B_SH) :
+  (SH_int ( bV₁ y t ( ¬₁((E₁ x A)∧₁B) ) ) (Recreate ({x}∪a∪g,b∪(c'),( bV₁ y t (A_SH ∨₁ (bE₁ c c' (substitution_formula d ((Term.var g)·(Term.var c)) B_SH)   )) )))) := by sorry
+-/
+
+
+-- ---------------------------------------------------------------------
+-- REMARK 2.4 (p.40):
+-- Interpretation of formulas with empty tuples
+-- ---------------------------------------------------------------------
+
+/-
+SH_int A AuSH
+AuSH.components = (a₁,a₂,A_SH)            -- ∀a ∃b A_SH(a,b)
+(hA : StarLang.isBase A_SH)
+
+SH_int B BuSH
+BuSH.components = (b₁,{},B_SH)            -- ∀b₁ B_SH(b₁)
+(hB : StarLang.isBase B_SH)
+
+SH_int C CuSH
+CuSH.components = ({},c₂,C_SH)            -- ∃c₂ A_SH(c₂)
+(hC : StarLang.isBase C_SH)
+-/
+
+example   -- B∨C
+  (hB1 : SH_int B BuSH) (hB2 : BuSH.components = (b₁,{},B_SH)) (hB3 : StarLang.isBase B_SH)
+  (hC1 : SH_int C CuSH) (hC2 : CuSH.components = ({},c₂,C_SH)) (hC3 : StarLang.isBase C_SH) :
+  (SH_int ( B∨₁C ) (Recreate (b₁,c₂,(B_SH ∨₁ C_SH)))) := by sorry
+
+example   -- ∀x B(x)
+  (hB1 : SH_int B BuSH) (hB2 : BuSH.components = (b₁,{},B_SH)) (hB3 : StarLang.isBase B_SH)
+  (x : String) :
+  (SH_int ( V₁ x B ) (Recreate ({x}∪b₁,{},B_SH))) := by sorry
+
+example   -- ∀x∈t C(x)
+  (hC1 : SH_int C CuSH) (hC2 : CuSH.components = ({},c₂,C_SH)) (hC3 : StarLang.isBase C_SH)
+  (x : String) (t : Term) :
+  (SH_int ( bV₁ x t C ) (Recreate ({},c₂,( bV₁ x t C_SH)))) := by sorry
+
+/- Problemma: Não funciona porque b₁ é tipo Finset String mas bE₁ só aceita String
+            -> Existe some upward arrow?
+
+lemma EmptyExistentialTuple (hB1 : SH_int B BuSH) (hB2 : BuSH.components = (b₁,{},B_SH)) (hB : StarLang.isBase B_SH) :
+  (  SH_int ( ¬₁ B ) ( Recreate ({},{b₁'},( bE₁ b₁ (b₁') (¬₁B_SH) ) ) )  ) := by sorry
+-/
+
+lemma EmptyUniversalTuple (hC1 : SH_int C CuSH) (hC2 : CuSH.components = ({},c₂,C_SH)) (hC : StarLang.isBase C_SH) :
+  (  SH_int ( ¬₁ C ) ( Recreate (c₂,{},(¬₁ C_SH ) ) )  ) := by sorry
+
+
+
+-- ---------------------------------------------------------------------
+-- EXAMPLE 2.3 (p.41-42):
+-- Interpretation of ∀x∈z ∃y A(x,y) → ∃w ∀x∈z ∃y∈w A(x,y)
+-- ---------------------------------------------------------------------
+
+-- TO DO / Problema yes: não consigo ter B = ... (both are formulas)
+
+lemma example_2_3
+  (hA1 : SH_int A AuSH) (hA2 : AuSH.components = ({},{},A_SH)) (hA3 : StarLang.isBase A_SH)
+  (B : Formula) (x y z w : String)
+  (H : B = (¬₁( bV₁ x (Term.var z) (¬₁(V₁ y (¬₁ A)))))∨₁(¬₁(V₁ w (¬₁(bV₁ x (Term.var z) (bE₁ y (Term.var w) A)))))) :
+  (SH_int B (Recreate ({y'},{w'},( (bV₁ x (Term.var z) (bE₁ y (Term.var y') A)) →₁ (bE₁ w (Term.var w') (bV₁ x (Term.var z) (bE₁ y (Term.var w) A)))  )))) := by sorry
+
+
+
+-- ---------------------------------------------------------------------
+-- EXAMPLE 2.4 (p.42-43):
+-- Interpretation of the bounded axiom of choice
+--     ∀x ∃y A_b(x,y) → ∃f ∀x ∃y∈fx A_b(x,y)
+-- ---------------------------------------------------------------------
+
+-- TO DO / Problema: não consigo ter B = ... (both are formulas)
+
+lemma int_bAC_ω_star
+  (hA1 : SH_int A AuSH) (hA2 : AuSH.components = ({},{},A_SH)) (hA3 : StarLang.isBase A_SH)
+  (B : Formula) (f x x' y y' a b f f' g Φ: String) :
+  --(B = ( (V₁ x (E₁ y A)) →₁ (E₁ f (V₁ x (bE₁ y ((Term.var f)·(Term.var x))) A))) ) ) :
+  (SH_int B (Recreate ({g,Φ},{x',f'},(  ( bV₁ x (Term.var x') (bE₁ y ((Term.var g)·(Term.var x)) A) ) →₁ ( bE₁ f (Term.var f')  (bV₁ a ((Term.var Φ)·(Term.var f)) (bE₁ b ((Term.var f)·(Term.var a)) A)) )  )))) := by sorry
+
+
+-- ---------------------------------------------------------------------
+-- PROPOSITION 2.1 (p.43):
+-- Interpretation of formulas with defined symbols
+-- ---------------------------------------------------------------------
+
+/- EXEMPLO BASE (a tirar depois)
+-- -- -- [-- tirar a partir daqui --] -- -- --
+example
+  (hA1 : SH_int A AuSH) (hA2 : AuSH.components = (a,b,A_SH)) (hA3 : StarLang.isBase A_SH)
+  (hB1 : SH_int B BuSH) (hB2 : BuSH.components = (c,d,B_SH)) (hB3 : StarLang.isBase B_SH) :
+  (SH_int (  ) (Recreate ( , , ))) := by sorry
+
+(substitution_formula b ((Term.var f)·(Term.var a)) A_SH)
+(substitution_formula d ((Term.var g)·(Term.var c)) B_SH)
+-- -- -- [-- tirar até aqui --] -- -- --
+
+lemma Int_DefinedSymbols_imp
+  (hA1 : SH_int A AuSH) (hA2 : AuSH.components = (a,b,A_SH)) (hA3 : StarLang.isBase A_SH)
+  (hB1 : SH_int B BuSH) (hB2 : BuSH.components = (c,d,B_SH)) (hB3 : StarLang.isBase B_SH)
+  (f : String):
+  (SH_int ( A →₁ B ) (Recreate (f∪c,(a')∪d, ((bV₁ a a' (substitution_formula b ((Term.var f)·(Term.var a)) A_SH)) →₁ B_SH) )) := by sorry
+
+lemma Int_DefinedSymbols_and      -- TO DO: incluir subst no A_SH
+  (hA1 : SH_int A AuSH) (hA2 : AuSH.components = (a,b,A_SH)) (hA3 : StarLang.isBase A_SH)
+  (hB1 : SH_int B BuSH) (hB2 : BuSH.components = (c,d,B_SH)) (hB3 : StarLang.isBase B_SH)
+  (f f' g g' Φ Ψ : String):
+  (SH_int ( A ∧₁ B ) (Recreate ({Φ,Ψ},{f',g'}, (bE₁ f (Term.var f') (bE₁ g (Term.var g') ((bV₁ a (((Term.var Φ)·(Term.var f))·(Term.var g)) (substitution_formula b ((Term.var f)·(Term.var a)) A_SH))∧₁(bV₁ c (((Term.var Ψ)·(Term.var f))·(Term.var g)) (substitution_formula d ((Term.var g)·(Term.var c)) B_SH))))) ))) := by sorry
+
+lemma Int_DefinedSymbols_unbExists      -- TO DO: incluir subst no A_SH
+  (hA1 : SH_int A AuSH) (hA2 : AuSH.components = (a,b,A_SH)) (hA3 : StarLang.isBase A_SH)
+  (hB1 : SH_int B BuSH) (hB2 : BuSH.components = (c,d,B_SH)) (hB3 : StarLang.isBase B_SH)
+  (x x' Φ f f': String):
+  (SH_int ( E₁ x A ) (Recreate ( {Φ} , {x',f'} , (bE₁ x (Term.var x') (bE₁ f (Term.var f') (bV₁ a (((Term.var Φ)·(Term.var x))·(Term.var f)) (substitution_formula b ((Term.var f)·(Term.var a)) A_SH)))) ))) := by sorry
+
+lemma Int_DefinedSymbols_bExists      -- TO DO: incluir subst no A_SH
+  (hA1 : SH_int A AuSH) (hA2 : AuSH.components = (a,b,A_SH)) (hA3 : StarLang.isBase A_SH)
+  (hB1 : SH_int B BuSH) (hB2 : BuSH.components = (c,d,B_SH)) (hB3 : StarLang.isBase B_SH)
+  (x Φ f f' : String) (t : Term):
+  (SH_int ( bE₁ x t A ) (Recreate ( {Φ} , {f'} , (bE₁ f (Term.var f') (bE₁ x t (bV₁ a ((Term.var Φ)·(Term.var f)) (substitution_formula b ((Term.var f)·(Term.var a)) A_SH) ))) ))) := by sorry
+
+
+
+
+Falta: 1. Escrever conclusões: done
+       2. Incluir substituições: done
+       3. Tentar fazer isTrue para capítulo 3? half done
+-/
+
+
+
+
+
+
+
+
+-- ---------------------------------------------------------------------
+-- REMARK 2.6 (p.45):
+-- For a given base formula A, the interpretation of ∃x A(x) is given by
+--            ∃x' [ ∃x∈x' A(x) ]
+-- ---------------------------------------------------------------------
+
+lemma Remark_2_6
+  (hA1 : SH_int A AuSH) (hA2 : AuSH.components = (a,b,A_SH)) (hA3 : StarLang.isBase A_SH)
+  (x x' : String) :
+  (SH_int ( E₁ x A ) (Recreate ({},{x'}, (bE₁ x (Term.var x') A) ))) := by sorry
+
+
+-- ---------------------------------------------------------------------
+-- REMARK 2.7 (p.45):
+-- Interpretations of formulas of the form ∃x A(x) with empty tuples
+-- ---------------------------------------------------------------------
+
+/-
+SH_int A AuSH
+AuSH.components = (a₁,a₂,A_SH)            -- ∀a ∃b A_SH(a,b)
+(hA : StarLang.isBase A_SH)
+
+SH_int B BuSH
+BuSH.components = (a,{},B_SH)             -- ∀a B_SH(a)
+(hB : StarLang.isBase B_SH)
+
+SH_int C CuSH
+CuSH.components = ({},b,C_SH)            -- ∃b C_SH(b)
+(hC : StarLang.isBase C_SH)
+
+-- Problema: same as before: a has type Finset String, mas bV₁ aceita String
+lemma Remark_2_7_1
+  (hB1 : SH_int B BuSH) (hB2 : BuSH.components = (a,{},B_SH)) (hB3 : StarLang.isBase B_SH)
+  (x x' Φ : String) :
+  (SH_int ( E₁ x B ) (Recreate ({Φ},{x'}, (bE₁ x (Term.var x') (bV₁ a ((Term.var Φ)·(Term.var x)) B)) ))) := by sorry
+
+-- Problema: same as before: a has type Finset String, mas bE₁ aceita String
+lemma Remark_2_7_2
+  (hC1 : SH_int C CuSH) (hC2 : BuSH.components = ({},b,C_SH)) (hC3 : StarLang.isBase C_SH)
+  (x x' b' : String) :
+  (SH_int ( E₁ x C ) (Recreate ({},{x',b}, (bE₁ x (Term.var x') (bE₁ b b' C)) ))) := by sorry
+-/
+
+
+-- ---------------------------------------------------------------------
+-- EXAMPLE 2.5 (p.45-46): Example 2.4 revisited
+-- Interpretation of the bounded axiom of choice
+--     ∀x ∃y A_b(x,y) → ∃f ∀a ∃b∈fa A_b(a,b)
+-- ---------------------------------------------------------------------
+
+-- TO DO (eu): copiar enunciado do Example 2.4 para depois prove with previous remarks
