LeanProjeto2/Sect31Soundness.lean
@@ -1,0 +1,100 @@
+import LeanProjeto2.FOL
+import LeanProjeto2.StarLang
+import LeanProjeto2.ShoenfieldsFunctInterp
+import MathLib.Tactic
+import Mathlib.Data.Finset.Basic
+import Mathlib.Data.Multiset.Basic
+
+open FOL
+open LFormula
+open StarLang
+
+-- ---------------------------------------------------------------------------------------------------------------
+-- ---------------------------------------------------------------------------------------------------------------
+--             SECTION 3: THE SOUNDNESS THEOREM AND OTHER RESULTS
+-- ---------------------------------------------------------------------------------------------------------------
+-- ---------------------------------------------------------------------------------------------------------------
+
+/- EXEMPLO BASE (a tirar depois)
+-- -- -- [-- tirar a partir daqui --] -- -- --
+example
+  (hA1 : SH_int A AuSH) (hA2 : AuSH.components = (a,b,A_SH)) (hA3 : StarLang.isBase A_SH)
+  (hB1 : SH_int B BuSH) (hB2 : BuSH.components = (c,d,B_SH)) (hB3 : StarLang.isBase B_SH) :
+  (SH_int (  ) (Recreate ( , , ))) := by sorry
+
+(substitution_formula b ((Term.var f)·(Term.var a)) A_SH)
+(substitution_formula d ((Term.var g)·(Term.var c)) B_SH)
+-- -- -- [-- tirar até aqui --] -- -- --
+-/
+
+
+
+-- ---------------------------------------------------------------------------------------------------------------
+--                     SECTION 3.1: The Soundness theorem
+-- ---------------------------------------------------------------------------------------------------------------
+
+-- ---------------------------------------------------------------------
+-- LEMMA 3.1 (p.48):
+-- Monotonicity lemma
+-- ---------------------------------------------------------------------
+
+/-
+-- Problema / TODO: o ∈₁ e o =₁ também têm de ser para Finset String :(
+def inclusion_symbol (x b b' : Finset String) : Formula :=
+  (V₁ x ((x ∈₁ b) →₁ (x ∈₁ b')))
+
+notation x "⊆₁" y => inclusion_symbol x y
+
+lemma MonotonicityLemma
+  (A : Formula) (b b' : Finset String)
+  (hA1 : SH_int A AuSH) (hA2 : AuSH.components = (a,b,A_SH)) (hA3 : StarLang.isBase A_SH) :
+  isTrue (((b ⊆₁ b') ∧₁ A_SH) →₁ (substitution_formula b b' A_SH)) := by sorry
+
+-/
+
+-- ---------------------------------------------------------------------
+-- THEOREM 3.1 (p.49):
+-- Soundness theorem
+-- ---------------------------------------------------------------------
+
+-- TO DO: Tem de ser o enunciado geral -> Ref Remark 3.2 (p.49)
+-- Problema: Como fazer isTrue com bAC to give A? O que está escrito doesn't work, to prove a conclusão, não precisamos de bAC
+
+/- Problema: same as before com String e Finset String
+theorem SoundnessTheorem
+  (A : Formula) (t : Term)
+  (hA1 : SH_int A AuSH) (hA2 : AuSH.components = (a,b,A_SH)) (hA3 : StarLang.isBase A_SH) :
+  (isTrue A) →
+  (isTrue.bAC) →
+  (isTrue (V₁ a (substitution_formula b (t·(Term.var a)) A_SH))) := by sorry
+-/
+
+
+-- ---------------------------------------------------------------------
+-- EXAMPLE 3.1 (p.49-50):
+-- Continuation of example 2.3 - Applying the soundness theorem
+-- ---------------------------------------------------------------------
+
+-- TO DO (eu): quando example 2.3 estiver bem enunciado
+
+
+-- ---------------------------------------------------------------------
+-- EXAMPLE 3.2 (p.50): The soundness theorem applied to bAC_ω_star
+-- Continuation of example 2.4 - Applying the soundness theorem
+-- ---------------------------------------------------------------------
+
+-- TO DO (eu): quando example 2.4 estiver bem enunciado
+
+
+-- ---------------------------------------------------------------------
+-- REMARK 3.3 (p.51):
+-- Soundness theorem for universal closure of base formulas
+-- ---------------------------------------------------------------------
+
+
+
+
+-- ---------------------------------------------------------------------
+-- REMARK 3.4 (p.56-57):
+-- Typechecking of the types in the soundness theorem
+-- ---------------------------------------------------------------------
