LeanProjeto2/Sect32ChrThm.lean
@@ -1,0 +1,135 @@
+import LeanProjeto2.FOL
+import LeanProjeto2.StarLang
+import LeanProjeto2.ShoenfieldsFunctInterp
+import LeanProjeto2.Sect31Soundness
+import MathLib.Tactic
+import Mathlib.Data.Finset.Basic
+import Mathlib.Data.Multiset.Basic
+
+open FOL
+open LFormula
+open StarLang
+
+
+-- ---------------------------------------------------------------------------------------------------------------
+--                     SECTION 3.2: Further results
+-- ---------------------------------------------------------------------------------------------------------------
+
+-- ---------------------------------------------------------------------------------------------------------------
+--          SUBSECTION 3.2.1: The characterization theorem
+-- ---------------------------------------------------------------------------------------------------------------
+
+-- ---------------------------------------------------------------------
+-- THEOREM 3.2 (p.58):
+-- Characterization theorem
+-- ---------------------------------------------------------------------
+
+-- Problema: why is (H2 : isTrue.bAC) not working while H is? Plus we have {x y f : String} in the assumption...
+theorem CharacterizationTheorem
+  (A : Formula) {x y f : String}
+  (hA1 : SH_int A AuSH) (hA2 : AuSH.components = (a,b,A_SH)) (hA3 : StarLang.isBase A_SH)
+  (H : isTrue ((V₁ x (E₁ y A)) →₁ (E₁ f (V₁ x (bE₁ y ((Term.var f)·(Term.var x)) A))))) :
+  --(H2 : isTrue.bAC ):
+  (isTrue (A ↔₁ AuSH)) := by sorry
+
+-- ---------------------------------------------------------------------
+-- LEMMA 3.2 (p.58):
+-- Principle 1
+-- ---------------------------------------------------------------------
+
+-- TODO / Problema: falta o bAC as assumption
+lemma LemmaPrinciple1
+  (A : Formula) (hA : isBase A) (x y b : String) (t : Term) :
+  (isTrue ((bV₁ x t (E₁ y A)) →₁ (E₁ b (bV₁ x t (bE₁ y (Term.var b) A))))) := by sorry
+
+
+-- ---------------------------------------------------------------------
+-- LEMMA 3.3 (p.58):
+-- Principle 2
+-- ---------------------------------------------------------------------
+
+-- TODO: falta o bAC as assumption
+lemma LemmaPrinciple2
+  (A : Formula) (hA : isBase A) (x y g : String) (t : Term) :
+  (isTrue ((V₁ x (E₁ y A)) →₁ (E₁ g (V₁ x (substitution_formula y ((Term.var g)·(Term.var x)) A))))) := by sorry
+
+
+-- ---------------------------------------------------------------------------------------------------------------
+--          SUBSECTION 3.2.2: Characteristic principles
+-- ---------------------------------------------------------------------------------------------------------------
+
+-- ---------------------------------------------------------------------
+-- REMARK 3.7 (p.60):
+-- Minimal collection of principles in the soundness theorem
+-- ---------------------------------------------------------------------
+
+-- Como formular? Vale a pena formular?
+
+
+-- ---------------------------------------------------------------------------------------------------------------
+--          SUBSECTION 3.2.3: Relation between Herbrand's thm and the soundness thm
+-- ---------------------------------------------------------------------------------------------------------------
+
+-- ---------------------------------------------------------------------
+-- THEOREM 3.3 (p.61):
+-- Herbrand's theorem
+-- ---------------------------------------------------------------------
+
+-- TO DO (eu): é preciso criar isTrue em PL (FOL)
+
+
+-- ---------------------------------------------------------------------
+-- THEOREM 3.4 (p.62):
+-- Main theorem
+-- ---------------------------------------------------------------------
+
+/- Problema: Why isn't (ht : isClosedTerm t) working?
+theorem MainTheorem
+  (A : Formula) (x : String) (t : Term)
+  (ht : isClosedTerm t) :
+  (isTrue (E₁ x A)) → (∃t, isTrue (bE₁ x t A)) := by sorry
+-/
+
+-- Problemas:
+--    1. Falta o (ht : isClosedTerm t)
+--    2. Falta que (E₁ x A) é derivable in PL+bAC mas que (bE₁ x t A) é só em PL
+theorem MainTheorem   -- erros vieram daqui
+  (A : Formula) (x : String) (t : Term) (ht : t.isClosedTerm):
+  (isTrue (L := Logic.PL_bAC) (E₁ x A)) → (∃t, isTrue (L := Logic.PL) (bE₁ x t A)) := by sorry
+
+/-
+theorem MainTheorem2
+  (A : Formula) (x : String) (t : Term) :
+  ((E₁ x A) → (∃t, (bE₁ x t A))) := by sorry
+-/
+
+-- ---------------------------------------------------------------------
+-- COROLLARY 3.1 (p.62):
+-- General form of Herbrand's theorem
+-- ---------------------------------------------------------------------
+
+/- Problema: como fazer lista finita de termos para depois substitution com A(t₁)∨...∨A(tₙ)?
+theorem HerbrandGeneralForm
+  (A : Formula) (x : String) (t : Term) :
+  (isTrue (E₁ x A)) → ( ∃{t₁,...,tₙ}, isTrue (A(t₁)∨...∨A(tₙ)) ) := by sorry
+-/
+
+
+-- ---------------------------------------------------------------------
+-- COROLLARY 3.2 (p.62):
+-- Corollary of the main theorem
+-- ---------------------------------------------------------------------
+
+-- TO DO once Corollary 3.1 is fixed
+
+
+-- ---------------------------------------------------------------------
+-- LEMMA 3.4 (p.63):
+-- Closed terms of star type "represent disjunctions"
+-- ---------------------------------------------------------------------
+
+/- TO DO: this has to be done better
+Problema: como fazer (x=t₁)∨₁...∨₁(x=tₙ)?
+lemma Lemma3_4
+  isTrue (V₁ x ((x ∈₁ t) ↔₁ ((x=t₁)∨₁...∨₁(x=tₙ))))
+-/
