LeanProjeto2/Technicalities.lean
@@ -1,2 +1,0 @@
-import LeanProjeto2.FOL
-import LeanProjeto2.StarLang_old
