LeanProjeto2/testee.lean
@@ -1,0 +1,2 @@
+import LeanProjeto2.FOL
+import LeanProjeto2.StarLang
